code/ed25519/Hacl.Impl.Ed25519.Ladder.fst
@@ -12,9 +12,13 @@ module F51 = Hacl.Impl.Ed25519.Field51
 
 module LSeq = Lib.Sequence
 module BSeq = Lib.ByteSequence
+
+module LE = Lib.Exponentiation
 module SE = Spec.Exponentiation
 module BE = Hacl.Impl.Exponentiation
 module ME = Hacl.Impl.MultiExponentiation
+module PT = Hacl.Impl.PrecompTable
+module SPT = Hacl.Spec.PrecompBaseTable
 
 module BD = Hacl.Bignum.Definitions
 module BC = Hacl.Bignum.Convert
@@ -30,53 +34,18 @@ unfold
 let a_spec = S.aff_point_c
 
 unfold
-let lseq_as_felem (a:LSeq.lseq uint64 5) : GTot Hacl.Spec.Curve25519.Field51.Definition.felem5 =
-  let s0 = LSeq.index a 0 in
-  let s1 = LSeq.index a 1 in
-  let s2 = LSeq.index a 2 in
-  let s3 = LSeq.index a 3 in
-  let s4 = LSeq.index a 4 in
-  (s0, s1, s2, s3, s4)
-
-unfold
-let refl_ext_point (a:LSeq.lseq uint64 20) : GTot S.ext_point =
-  let open Hacl.Spec.Curve25519.Field51.Definition in
-  let x = feval (lseq_as_felem (LSeq.sub a 0 5)) in
-  let y = feval (lseq_as_felem (LSeq.sub a 5 5)) in
-  let z = feval (lseq_as_felem (LSeq.sub a 10 5)) in
-  let t = feval (lseq_as_felem (LSeq.sub a 15 5)) in
-  (x, y, z, t)
-
-unfold
-let inv_ext_point (a:LSeq.lseq uint64 20) : Type0 =
-  S.point_inv (refl_ext_point a)
-
-
-unfold
-let linv (a:LSeq.lseq uint64 20) : Type0 =
-  let open Hacl.Spec.Curve25519.Field51 in
-  mul_inv_t (lseq_as_felem (LSeq.sub a 0 5)) /\
-  mul_inv_t (lseq_as_felem (LSeq.sub a 5 5)) /\
-  mul_inv_t (lseq_as_felem (LSeq.sub a 10 5)) /\
-  mul_inv_t (lseq_as_felem (LSeq.sub a 15 5)) /\
-  inv_ext_point a
-
-
-unfold
-let refl (a:LSeq.lseq uint64 20{linv a}) : GTot a_spec =
-  S.to_aff_point (refl_ext_point a)
-
+let refl (a:LSeq.lseq uint64 20{F51.linv a}) : GTot a_spec =
+  S.to_aff_point (F51.refl_ext_point a)
 
 unfold
 let linv_ctx (a:LSeq.lseq uint64 0) : Type0 = True
-
 
 inline_for_extraction noextract
 let mk_to_ed25519_comm_monoid : BE.to_comm_monoid U64 20ul 0ul = {
   BE.a_spec = a_spec;
   BE.comm_monoid = S.mk_ed25519_comm_monoid;
   BE.linv_ctx = linv_ctx;
-  BE.linv = linv;
+  BE.linv = F51.linv;
   BE.refl = refl;
   }
 
@@ -85,7 +54,8 @@ inline_for_extraction noextract
 val point_add : BE.lmul_st U64 20ul 0ul mk_to_ed25519_comm_monoid
 let point_add ctx x y xy =
   let h0 = ST.get () in
-  Spec.Ed25519.Lemmas.to_aff_point_add_lemma (refl_ext_point (as_seq h0 x)) (refl_ext_point (as_seq h0 y));
+  Spec.Ed25519.Lemmas.to_aff_point_add_lemma
+    (F51.refl_ext_point (as_seq h0 x)) (F51.refl_ext_point (as_seq h0 y));
   Hacl.Impl.Ed25519.PointAdd.point_add xy x y
 
 
@@ -93,7 +63,7 @@ inline_for_extraction noextract
 val point_double : BE.lsqr_st U64 20ul 0ul mk_to_ed25519_comm_monoid
 let point_double ctx x xx =
   let h0 = ST.get () in
-  Spec.Ed25519.Lemmas.to_aff_point_double_lemma (refl_ext_point (as_seq h0 x));
+  Spec.Ed25519.Lemmas.to_aff_point_double_lemma (F51.refl_ext_point (as_seq h0 x));
   Hacl.Impl.Ed25519.PointDouble.point_double xx x
 
 
@@ -102,7 +72,7 @@ val make_point_inf:
   Stack unit
   (requires fun h -> live h b)
   (ensures  fun h0 _ h1 -> modifies (loc b) h0 h1 /\
-    F51.point_inv_t h1 b /\ inv_ext_point (as_seq h1 b) /\
+    F51.point_inv_t h1 b /\ F51.inv_ext_point (as_seq h1 b) /\
     S.to_aff_point (F51.point_eval h1 b) == S.aff_point_at_infinity)
 
 let make_point_inf b =
@@ -135,12 +105,73 @@ let mk_ed25519_concrete_ops : BE.concrete_ops U64 20ul 0ul = {
 //////////////////////////////////////////////
 
 inline_for_extraction noextract
-val make_g:
-  g:point ->
-  Stack unit
+val ext_point_to_list: p:S.ext_point_c
+  -> x:list uint64{FStar.List.Tot.length x = 20 /\
+    mk_to_ed25519_comm_monoid.BE.linv (Seq.seq_of_list x)}
+
+let ext_point_to_list p =
+  Hacl.Spec.Ed25519.PrecompTable.ext_point_to_list_lemma p;
+  Hacl.Spec.Ed25519.PrecompTable.ext_point_to_list p
+
+
+val lemma_refl: x:S.ext_point_c ->
+  Lemma (S.mk_ed25519_concrete_ops.SE.to.SE.refl x ==
+    mk_to_ed25519_comm_monoid.BE.refl (Seq.seq_of_list (ext_point_to_list x)))
+
+let lemma_refl x =
+  Hacl.Spec.Ed25519.PrecompTable.ext_point_to_list_eval x
+
+
+inline_for_extraction noextract
+let mk_ed25519_precomp_base_table: SPT.mk_precomp_base_table S.ext_point_c U64 20ul 0ul = {
+  SPT.concr_ops = S.mk_ed25519_concrete_ops;
+  SPT.to_cm = mk_to_ed25519_comm_monoid;
+  SPT.to_list = ext_point_to_list;
+  SPT.lemma_refl = lemma_refl;
+}
+
+inline_for_extraction noextract
+let g_c : S.ext_point_c =
+  Spec.Ed25519.Lemmas.g_is_on_curve ();
+  S.g
+
+unfold let precomp_basepoint_table_list: x:list uint64{FStar.List.Tot.length x = 320} =
+  normalize_term (SPT.precomp_base_table_list mk_ed25519_precomp_base_table g_c 15)
+
+inline_for_extraction noextract
+let precomp_basepoint_table_lseq : LSeq.lseq uint64 320 =
+  normalize_term_spec (SPT.precomp_base_table_list mk_ed25519_precomp_base_table g_c 15);
+  Seq.seq_of_list precomp_basepoint_table_list
+
+
+inline_for_extraction noextract
+let pow_base_point (k:nat) =
+  LE.pow S.mk_ed25519_comm_monoid (S.to_aff_point g_c) k
+
+unfold
+let precomp_table_acc_inv
+  (table_len:nat{table_len * 20 <= max_size_t})
+  (table:LSeq.lseq uint64 (table_len * 20))
+  (j:nat{j < table_len})
+=
+  Math.Lemmas.lemma_mult_lt_right 20 j table_len;
+  Math.Lemmas.lemma_mult_le_right 20 (j + 1) table_len;
+  let bj = LSeq.sub table (j * 20) 20 in
+  F51.linv bj /\ refl bj == pow_base_point j
+
+val precomp_basepoint_table_lemma: unit ->
+  Lemma (forall (i:nat{i < 16}). precomp_table_acc_inv 16 precomp_basepoint_table_lseq i)
+let precomp_basepoint_table_lemma () =
+  normalize_term_spec (SPT.precomp_base_table_list mk_ed25519_precomp_base_table g_c 15);
+  SPT.precomp_base_table_lemma mk_ed25519_precomp_base_table g_c 16 precomp_basepoint_table_lseq
+
+/////////////////////////////////////////////////////
+
+inline_for_extraction noextract
+val make_g: g:point -> Stack unit
   (requires fun h -> live h g)
   (ensures fun h0 _ h1 -> modifies (loc g) h0 h1 /\
-    F51.point_inv_t h1 g /\
+    F51.point_inv_t h1 g /\ F51.inv_ext_point (as_seq h1 g) /\
     F51.point_eval h1 g == S.g)
 
 let make_g g =
@@ -148,21 +179,43 @@ let make_g g =
   let gy = gety g in
   let gz = getz g in
   let gt = gett g in
-  make_u64_5 gx (u64 0x00062d608f25d51a) (u64 0x000412a4b4f6592a) (u64 0x00075b7171a4b31d) (u64 0x0001ff60527118fe) (u64 0x000216936d3cd6e5);
-  make_u64_5 gy (u64 0x0006666666666658) (u64 0x0004cccccccccccc) (u64 0x0001999999999999) (u64 0x0003333333333333) (u64 0x0006666666666666);
+
+  [@inline_let] let (x0, x1, x2, x3, x4) =
+    (u64 0x00062d608f25d51a,
+     u64 0x000412a4b4f6592a,
+     u64 0x00075b7171a4b31d,
+     u64 0x0001ff60527118fe,
+     u64 0x000216936d3cd6e5) in
+
+  [@inline_let] let (y0, y1, y2, y3, y4) =
+    (u64 0x0006666666666658,
+     u64 0x0004cccccccccccc,
+     u64 0x0001999999999999,
+     u64 0x0003333333333333,
+     u64 0x0006666666666666) in
+
+  [@inline_let] let (t0, t1, t2, t3, t4) =
+    (u64 0x00068ab3a5b7dda3,
+     u64 0x00000eea2a5eadbb,
+     u64 0x0002af8df483c27e,
+     u64 0x000332b375274732,
+     u64 0x00067875f0fd78b7) in
+
+  make_u64_5 gx x0 x1 x2 x3 x4;
+  make_u64_5 gy y0 y1 y2 y3 y4;
   make_one gz;
-  make_u64_5 gt (u64 0x00068ab3a5b7dda3) (u64 0x00000eea2a5eadbb) (u64 0x0002af8df483c27e) (u64 0x000332b375274732) (u64 0x00067875f0fd78b7);
+  make_u64_5 gt t0 t1 t2 t3 t4;
 
   (**) assert_norm (Spec.Ed25519.g_x ==
-    Hacl.Spec.Curve25519.Field51.Definition.as_nat5 (u64 0x00062d608f25d51a, u64 0x000412a4b4f6592a, u64 0x00075b7171a4b31d, u64 0x0001ff60527118fe, u64 0x000216936d3cd6e5) % Spec.Curve25519.prime);
+    Hacl.Spec.Curve25519.Field51.Definition.as_nat5 (x0, x1, x2, x3, x4) % Spec.Curve25519.prime);
   (**) assert_norm (Spec.Ed25519.g_y ==
-    Hacl.Spec.Curve25519.Field51.Definition.as_nat5 (u64 0x0006666666666658, u64 0x0004cccccccccccc, u64 0x0001999999999999, u64 0x0003333333333333, u64 0x0006666666666666) %
-      Spec.Curve25519.prime);
+    Hacl.Spec.Curve25519.Field51.Definition.as_nat5 (y0, y1, y2, y3, y4) % Spec.Curve25519.prime);
   (**) assert_norm (Mktuple4?._4 Spec.Ed25519.g ==
-    Hacl.Spec.Curve25519.Field51.Definition.as_nat5 (u64 0x00068ab3a5b7dda3, u64 0x00000eea2a5eadbb, u64 0x0002af8df483c27e, u64 0x000332b375274732, u64 0x00067875f0fd78b7) % Spec.Curve25519.prime);
+    Hacl.Spec.Curve25519.Field51.Definition.as_nat5 (t0, t1, t2, t3, t4) % Spec.Curve25519.prime);
   let h1 = ST.get () in
   assert (F51.point_inv_t h1 g);
-  assert (F51.point_eval h1 g == Spec.Ed25519.g)
+  assert (F51.point_eval h1 g == Spec.Ed25519.g);
+  Spec.Ed25519.Lemmas.g_is_on_curve ()
 
 
 inline_for_extraction noextract
@@ -178,143 +231,319 @@ let convert_scalar scalar bscalar =
   Hacl.Bignum.Convert.mk_bn_from_bytes_le true 32ul scalar bscalar
 
 
+inline_for_extraction noextract
+val point_mul_noalloc:
+    out:point
+  -> bscalar:lbuffer uint64 4ul
+  -> q:point ->
+  Stack unit
+  (requires fun h ->
+    live h bscalar /\ live h q /\ live h out /\
+    disjoint q out /\ disjoint q bscalar /\ disjoint out bscalar /\
+    F51.point_inv_t h q /\ F51.inv_ext_point (as_seq h q) /\
+    BD.bn_v h bscalar < pow2 256)
+  (ensures  fun h0 _ h1 -> modifies (loc out) h0 h1 /\
+    F51.point_inv_t h1 out /\ F51.inv_ext_point (as_seq h1 out) /\
+    S.to_aff_point (F51.point_eval h1 out) ==
+    LE.exp_fw S.mk_ed25519_comm_monoid
+      (S.to_aff_point (F51.point_eval h0 q)) 256 (BD.bn_v h0 bscalar) 4)
+
+let point_mul_noalloc out bscalar q =
+  BE.lexp_fw_consttime 20ul 0ul mk_ed25519_concrete_ops
+    4ul (null uint64) q 4ul 256ul bscalar out
+
+
 val point_mul:
-    result:point
+    out:point
   -> scalar:lbuffer uint8 32ul
   -> q:point ->
   Stack unit
   (requires fun h ->
-    live h scalar /\ live h q /\ live h result /\
-    disjoint q result /\ disjoint q scalar /\
-    F51.point_inv_t h q /\ inv_ext_point (as_seq h q))
-  (ensures  fun h0 _ h1 -> modifies (loc result) h0 h1 /\
-    F51.point_inv_t h1 result /\ inv_ext_point (as_seq h1 result) /\
-    S.to_aff_point (F51.point_eval h1 result) ==
+    live h scalar /\ live h q /\ live h out /\
+    disjoint q out /\ disjoint q scalar /\
+    F51.point_inv_t h q /\ F51.inv_ext_point (as_seq h q))
+  (ensures  fun h0 _ h1 -> modifies (loc out) h0 h1 /\
+    F51.point_inv_t h1 out /\ F51.inv_ext_point (as_seq h1 out) /\
+    S.to_aff_point (F51.point_eval h1 out) ==
     S.to_aff_point (S.point_mul (as_seq h0 scalar) (F51.point_eval h0 q)))
 
-let point_mul result scalar q =
+let point_mul out scalar q =
   let h0 = ST.get () in
   SE.exp_fw_lemma S.mk_ed25519_concrete_ops
     (F51.point_eval h0 q) 256 (BSeq.nat_from_bytes_le (as_seq h0 scalar)) 4;
   push_frame ();
   let bscalar = create 4ul (u64 0) in
   convert_scalar scalar bscalar;
-  BE.lexp_fw_consttime 20ul 0ul mk_ed25519_concrete_ops 4ul (null uint64) q 4ul 256ul bscalar result;
+  point_mul_noalloc out bscalar q;
   pop_frame ()
+
+////////////////////////////////////////
+
+inline_for_extraction noextract
+let table_inv : BE.table_inv_t U64 20ul 16ul =
+  [@inline_let] let len = 20ul in
+  [@inline_let] let ctx_len = 0ul in
+  [@inline_let] let k = mk_ed25519_concrete_ops in
+  [@inline_let] let l = 4ul in
+  [@inline_let] let table_len = 16ul in
+  BE.table_inv_precomp len ctx_len k l table_len
+
+
+let precomp_basepoint_table:
+  x:glbuffer uint64 320ul{witnessed x precomp_basepoint_table_lseq /\ recallable x} =
+  createL_global precomp_basepoint_table_list
+
+
+inline_for_extraction noextract
+val point_mul_g_noalloc:
+    out:point
+  -> bscalar:lbuffer uint64 4ul
+  -> g:point -> Stack unit
+  (requires fun h ->
+    live h out /\ live h g /\ live h bscalar /\
+    disjoint out g /\ disjoint bscalar out /\ disjoint bscalar g /\
+    F51.point_inv_t h g /\ F51.inv_ext_point (as_seq h g) /\
+    F51.point_eval h g == g_c /\ BD.bn_v h bscalar < pow2 256)
+  (ensures  fun h0 _ h1 -> modifies (loc out) h0 h1 /\
+    F51.point_inv_t h1 out /\ F51.inv_ext_point (as_seq h1 out) /\
+    S.to_aff_point (F51.point_eval h1 out) ==
+    LE.exp_fw S.mk_ed25519_comm_monoid
+      (S.to_aff_point (F51.point_eval h0 g)) 256 (BD.bn_v h0 bscalar) 4)
+
+let point_mul_g_noalloc out bscalar g =
+  [@inline_let] let len = 20ul in
+  [@inline_let] let ctx_len = 0ul in
+  [@inline_let] let k = mk_ed25519_concrete_ops in
+  [@inline_let] let l = 4ul in
+  [@inline_let] let table_len = 16ul in
+  [@inline_let] let bLen = 4ul in
+  [@inline_let] let bBits = 256ul in
+
+  let h0 = ST.get () in
+  recall_contents precomp_basepoint_table precomp_basepoint_table_lseq;
+  let h1 = ST.get () in
+  precomp_basepoint_table_lemma ();
+  assert (table_inv (as_seq h1 g) (as_seq h1 precomp_basepoint_table));
+  assert (F51.point_eval h1 g == g_c);
+
+  BE.mk_lexp_fw_table len ctx_len k l table_len
+    table_inv
+    (BE.lprecomp_get_consttime len ctx_len k l table_len)
+    (null uint64) g bLen bBits bscalar (to_const precomp_basepoint_table) out
 
 
 val point_mul_g:
-    result:point
+    out:point
   -> scalar:lbuffer uint8 32ul ->
   Stack unit
   (requires fun h ->
-    live h scalar /\ live h result /\ disjoint result scalar)
-  (ensures  fun h0 _ h1 -> modifies (loc result) h0 h1 /\
-    F51.point_inv_t h1 result /\ inv_ext_point (as_seq h1 result) /\
-    S.to_aff_point (F51.point_eval h1 result) ==
+    live h scalar /\ live h out /\ disjoint out scalar)
+  (ensures  fun h0 _ h1 -> modifies (loc out) h0 h1 /\
+    F51.point_inv_t h1 out /\ F51.inv_ext_point (as_seq h1 out) /\
+    S.to_aff_point (F51.point_eval h1 out) ==
     S.to_aff_point (S.point_mul_g (as_seq h0 scalar)))
 
 [@CInline]
-let point_mul_g result scalar =
+let point_mul_g out scalar =
+  let h0 = ST.get () in
+  SE.exp_fw_lemma S.mk_ed25519_concrete_ops
+    g_c 256 (BSeq.nat_from_bytes_le (as_seq h0 scalar)) 4;
+
   push_frame ();
   let g = create 20ul (u64 0) in
   make_g g;
-  Spec.Ed25519.Lemmas.g_is_on_curve ();
-  point_mul result scalar g;
+
+  let bscalar = create 4ul (u64 0) in
+  convert_scalar scalar bscalar;
+  point_mul_g_noalloc out bscalar g;
   pop_frame ()
 
 
-#push-options "--z3rlimit 150"
-val point_mul_double_vartime:
-    result:point
-  -> scalar1:lbuffer uint8 32ul
-  -> q1:point
-  -> scalar2:lbuffer uint8 32ul
-  -> q2:point ->
+inline_for_extraction noextract
+val point_mul_g_double_vartime_noalloc:
+    out:point
+  -> scalar1:lbuffer uint64 4ul -> q1:point
+  -> scalar2:lbuffer uint64 4ul -> q2:point
+  -> table2: lbuffer uint64 320ul ->
   Stack unit
   (requires fun h ->
-    live h result /\ live h scalar1 /\ live h q1 /\
-    live h scalar2 /\ live h q2 /\
-    disjoint q1 result /\ disjoint q2 result /\
-    disjoint q1 q2 /\
-    F51.point_inv_t h q1 /\ inv_ext_point (as_seq h q1) /\
-    F51.point_inv_t h q2 /\ inv_ext_point (as_seq h q2))
-  (ensures fun h0 _ h1 -> modifies (loc result) h0 h1 /\
-    F51.point_inv_t h1 result /\ inv_ext_point (as_seq h1 result) /\
-    S.to_aff_point (F51.point_eval h1 result) ==
-    S.to_aff_point (S.point_mul_double
-      (as_seq h0 scalar1) (F51.point_eval h0 q1)
-      (as_seq h0 scalar2) (F51.point_eval h0 q2)))
+    live h out /\ live h scalar1 /\ live h q1 /\
+    live h scalar2 /\ live h q2 /\ live h table2 /\
 
-[@CInline]
-let point_mul_double_vartime result scalar1 q1 scalar2 q2 =
+    eq_or_disjoint q1 q2 /\ disjoint out q1 /\ disjoint out q2 /\
+    disjoint out scalar1 /\ disjoint out scalar2 /\ disjoint out table2 /\
+
+    BD.bn_v h scalar1 < pow2 256 /\ BD.bn_v h scalar2 < pow2 256 /\
+    F51.point_inv_t h q1 /\ F51.inv_ext_point (as_seq h q1) /\
+    F51.point_eval h q1 == g_c /\
+    F51.point_inv_t h q2 /\ F51.inv_ext_point (as_seq h q2) /\
+    table_inv (as_seq h q2) (as_seq h table2))
+  (ensures fun h0 _ h1 -> modifies (loc out) h0 h1 /\
+    F51.point_inv_t h1 out /\ F51.inv_ext_point (as_seq h1 out) /\
+    S.to_aff_point (F51.point_eval h1 out) ==
+    LE.exp_double_fw #S.aff_point_c S.mk_ed25519_comm_monoid
+      (S.to_aff_point (F51.point_eval h0 q1)) 256 (BD.bn_v h0 scalar1)
+      (S.to_aff_point (F51.point_eval h0 q2)) (BD.bn_v h0 scalar2) 4)
+
+let point_mul_g_double_vartime_noalloc out scalar1 q1 scalar2 q2 table2 =
+  [@inline_let] let len = 20ul in
+  [@inline_let] let ctx_len = 0ul in
+  [@inline_let] let k = mk_ed25519_concrete_ops in
+  [@inline_let] let l = 4ul in
+  [@inline_let] let table_len = 16ul in
+  [@inline_let] let bLen = 4ul in
+  [@inline_let] let bBits = 256ul in
+
   let h0 = ST.get () in
-  SE.exp_double_fw_lemma S.mk_ed25519_concrete_ops
-    (F51.point_eval h0 q1) 256 (BSeq.nat_from_bytes_le (as_seq h0 scalar1))
-    (F51.point_eval h0 q2) (BSeq.nat_from_bytes_le (as_seq h0 scalar2)) 4;
+  recall_contents precomp_basepoint_table precomp_basepoint_table_lseq;
+  let h1 = ST.get () in
+  precomp_basepoint_table_lemma ();
+  assert (table_inv (as_seq h1 q1) (as_seq h1 precomp_basepoint_table));
+  assert (table_inv (as_seq h1 q2) (as_seq h1 table2));
+
+  ME.mk_lexp_double_fw_tables len ctx_len k l table_len
+    table_inv table_inv
+    (BE.lprecomp_get_vartime len ctx_len k l table_len)
+    (BE.lprecomp_get_vartime len ctx_len k l table_len)
+    (null uint64) q1 bLen bBits scalar1 q2 scalar2
+    (to_const precomp_basepoint_table) (to_const table2) out
+
+
+inline_for_extraction noextract
+val point_mul_g_double_vartime_table:
+    out:point
+  -> scalar1:lbuffer uint64 4ul -> q1:point
+  -> scalar2:lbuffer uint64 4ul -> q2:point ->
+  Stack unit
+  (requires fun h ->
+    live h out /\ live h scalar1 /\ live h q1 /\
+    live h scalar2 /\ live h q2 /\
+
+    eq_or_disjoint q1 q2 /\ disjoint out q1 /\ disjoint out q2 /\
+    disjoint out scalar1 /\ disjoint out scalar2 /\
+
+    BD.bn_v h scalar1 < pow2 256 /\ BD.bn_v h scalar2 < pow2 256 /\
+    F51.point_inv_t h q1 /\ F51.inv_ext_point (as_seq h q1) /\
+    F51.point_eval h q1 == g_c /\
+    F51.point_inv_t h q2 /\ F51.inv_ext_point (as_seq h q2))
+  (ensures fun h0 _ h1 -> modifies (loc out) h0 h1 /\
+    F51.point_inv_t h1 out /\ F51.inv_ext_point (as_seq h1 out) /\
+    S.to_aff_point (F51.point_eval h1 out) ==
+    LE.exp_double_fw #S.aff_point_c S.mk_ed25519_comm_monoid
+      (S.to_aff_point (F51.point_eval h0 q1)) 256 (BD.bn_v h0 scalar1)
+      (S.to_aff_point (F51.point_eval h0 q2)) (BD.bn_v h0 scalar2) 4)
+
+let point_mul_g_double_vartime_table out scalar1 q1 scalar2 q2 =
+  [@inline_let] let len = 20ul in
+  [@inline_let] let ctx_len = 0ul in
+  [@inline_let] let k = mk_ed25519_concrete_ops in
+  [@inline_let] let table_len = 16ul in
 
   push_frame ();
-  let bscalar1 = create 4ul (u64 0) in
-  convert_scalar scalar1 bscalar1;
+  let table2 = create (table_len *! len) (u64 0) in
+  PT.lprecomp_table len ctx_len k (null uint64) q2 table_len table2;
 
-  let bscalar2 = create 4ul (u64 0) in
-  convert_scalar scalar2 bscalar2;
-
-  ME.lexp_double_fw_vartime 20ul 0ul mk_ed25519_concrete_ops 4ul (null uint64) q1 4ul 256ul bscalar1 q2 bscalar2 result;
+  point_mul_g_double_vartime_noalloc out scalar1 q1 scalar2 q2 table2;
   pop_frame ()
-#pop-options
+
+
+inline_for_extraction noextract
+val point_mul_g_double_vartime_aux:
+    out:point
+  -> scalar1:lbuffer uint8 32ul -> q1:point
+  -> scalar2:lbuffer uint8 32ul -> q2:point
+  -> bscalar1:lbuffer uint64 4ul
+  -> bscalar2:lbuffer uint64 4ul ->
+  Stack unit
+  (requires fun h ->
+    live h out /\ live h scalar1 /\ live h q1 /\
+    live h scalar2 /\ live h q2 /\ live h bscalar1 /\ live h bscalar2 /\
+
+    disjoint scalar1 bscalar1 /\ disjoint scalar2 bscalar2 /\ disjoint scalar2 bscalar1 /\
+    disjoint scalar1 bscalar2 /\ disjoint bscalar1 bscalar2 /\ disjoint bscalar1 out /\
+    disjoint bscalar1 q1 /\ disjoint bscalar1 q2 /\ disjoint bscalar2 out /\
+    disjoint bscalar2 q1 /\ disjoint bscalar2 q2 /\ eq_or_disjoint q1 q2 /\
+    disjoint q1 out /\ disjoint q2 out /\ disjoint scalar1 out /\ disjoint scalar2 out /\
+
+    F51.point_inv_t h q1 /\ F51.inv_ext_point (as_seq h q1) /\
+    F51.point_eval h q1 == g_c /\
+    F51.point_inv_t h q2 /\ F51.inv_ext_point (as_seq h q2))
+  (ensures fun h0 _ h1 -> modifies (loc out |+| loc bscalar1 |+| loc bscalar2) h0 h1 /\
+    F51.point_inv_t h1 out /\ F51.inv_ext_point (as_seq h1 out) /\
+    BD.bn_v h1 bscalar1 == BSeq.nat_from_bytes_le (as_seq h0 scalar1) /\
+    BD.bn_v h1 bscalar2 == BSeq.nat_from_bytes_le (as_seq h0 scalar2) /\
+    S.to_aff_point (F51.point_eval h1 out) ==
+    LE.exp_double_fw #S.aff_point_c S.mk_ed25519_comm_monoid
+      (S.to_aff_point (F51.point_eval h0 q1)) 256 (BD.bn_v h1 bscalar1)
+      (S.to_aff_point (F51.point_eval h0 q2)) (BD.bn_v h1 bscalar2) 4)
+
+let point_mul_g_double_vartime_aux out scalar1 q1 scalar2 q2 bscalar1 bscalar2 =
+  let h0 = ST.get () in
+  convert_scalar scalar1 bscalar1;
+  convert_scalar scalar2 bscalar2;
+  let h1 = ST.get () in
+  assert (BD.bn_v h1 bscalar1 == BSeq.nat_from_bytes_le (as_seq h0 scalar1));
+  assert (BD.bn_v h1 bscalar2 == BSeq.nat_from_bytes_le (as_seq h0 scalar2));
+  point_mul_g_double_vartime_table out bscalar1 q1 bscalar2 q2
 
 
 val point_mul_g_double_vartime:
-    result:point
+    out:point
   -> scalar1:lbuffer uint8 32ul
   -> scalar2:lbuffer uint8 32ul
   -> q2:point ->
   Stack unit
   (requires fun h ->
-    live h result /\ live h scalar1 /\
+    live h out /\ live h scalar1 /\
     live h scalar2 /\ live h q2 /\
-    disjoint q2 result /\
-    F51.point_inv_t h q2 /\ inv_ext_point (as_seq h q2))
-  (ensures fun h0 _ h1 -> modifies (loc result) h0 h1 /\
-    F51.point_inv_t h1 result /\ inv_ext_point (as_seq h1 result) /\
-    S.to_aff_point (F51.point_eval h1 result) ==
-    S.to_aff_point (S.point_mul_double_g
-      (as_seq h0 scalar1) (as_seq h0 scalar2) (F51.point_eval h0 q2)))
+    disjoint q2 out /\ disjoint scalar1 out /\ disjoint scalar2 out /\
+    F51.point_inv_t h q2 /\ F51.inv_ext_point (as_seq h q2))
+  (ensures fun h0 _ h1 -> modifies (loc out) h0 h1 /\
+    F51.point_inv_t h1 out /\ F51.inv_ext_point (as_seq h1 out) /\
+    S.to_aff_point (F51.point_eval h1 out) ==
+    LE.exp_double_fw #S.aff_point_c S.mk_ed25519_comm_monoid
+      (S.to_aff_point g_c) 256 (BSeq.nat_from_bytes_le (as_seq h0 scalar1))
+      (S.to_aff_point (F51.point_eval h0 q2)) (BSeq.nat_from_bytes_le (as_seq h0 scalar2)) 4)
 
 [@CInline]
-let point_mul_g_double_vartime result scalar1 scalar2 q2 =
+let point_mul_g_double_vartime out scalar1 scalar2 q2 =
   push_frame ();
   let g = create 20ul (u64 0) in
   make_g g;
-  Spec.Ed25519.Lemmas.g_is_on_curve ();
-  point_mul_double_vartime result scalar1 g scalar2 q2;
+
+  let bscalar1 = create 4ul (u64 0) in
+  let bscalar2 = create 4ul (u64 0) in
+  point_mul_g_double_vartime_aux out scalar1 g scalar2 q2 bscalar1 bscalar2;
   pop_frame ()
 
 
 val point_negate_mul_double_g_vartime:
-    result:point
+    out:point
   -> scalar1:lbuffer uint8 32ul
   -> scalar2:lbuffer uint8 32ul
   -> q2:point ->
   Stack unit
   (requires fun h ->
-    live h result /\ live h scalar1 /\
+    live h out /\ live h scalar1 /\
     live h scalar2 /\ live h q2 /\
-    disjoint q2 result /\
-    F51.point_inv_t h q2 /\ inv_ext_point (as_seq h q2))
-  (ensures fun h0 _ h1 -> modifies (loc result) h0 h1 /\
-    F51.point_inv_t h1 result /\ inv_ext_point (as_seq h1 result) /\
-    S.to_aff_point (F51.point_eval h1 result) ==
+    disjoint q2 out /\ disjoint scalar1 out /\ disjoint scalar2 out /\
+    F51.point_inv_t h q2 /\ F51.inv_ext_point (as_seq h q2))
+  (ensures fun h0 _ h1 -> modifies (loc out) h0 h1 /\
+    F51.point_inv_t h1 out /\ F51.inv_ext_point (as_seq h1 out) /\
+    S.to_aff_point (F51.point_eval h1 out) ==
     S.to_aff_point (S.point_negate_mul_double_g
       (as_seq h0 scalar1) (as_seq h0 scalar2) (F51.point_eval h0 q2)))
 
 [@CInline]
-let point_negate_mul_double_g_vartime result scalar1 scalar2 q2 =
+let point_negate_mul_double_g_vartime out scalar1 scalar2 q2 =
   push_frame ();
   let q2_neg = create 20ul (u64 0) in
   let h0 = ST.get () in
-  Spec.Ed25519.Lemmas.to_aff_point_negate (refl_ext_point (as_seq h0 q2));
+  Spec.Ed25519.Lemmas.to_aff_point_negate (F51.refl_ext_point (as_seq h0 q2));
   Hacl.Impl.Ed25519.PointNegate.point_negate q2 q2_neg;
-  point_mul_g_double_vartime result scalar1 scalar2 q2_neg;
+  let h1 = ST.get () in
+  point_mul_g_double_vartime out scalar1 scalar2 q2_neg;
+  SE.exp_double_fw_lemma S.mk_ed25519_concrete_ops
+    g_c 256 (BSeq.nat_from_bytes_le (as_seq h1 scalar1))
+    (F51.point_eval h1 q2_neg) (BSeq.nat_from_bytes_le (as_seq h1 scalar2)) 4;
   pop_frame ()
