code/ed25519/Hacl.Spec.Ed25519.PrecompTable.fst
@@ -1,0 +1,259 @@
+module Hacl.Spec.Ed25519.PrecompTable
+
+open FStar.Mul
+open Lib.IntTypes
+open Lib.Sequence
+
+module F51 = Hacl.Impl.Ed25519.Field51
+module SF51 = Hacl.Spec.Curve25519.Field51.Definition
+
+module S = Spec.Ed25519
+module SC = Spec.Curve25519
+module FL = FStar.List.Tot
+module SPT = Hacl.Spec.PrecompBaseTable
+
+#set-options "--z3rlimit 50 --fuel 0 --ifuel 0"
+
+unfold
+let create5 (x0 x1 x2 x3 x4:uint64) : list uint64 = [x0; x1; x2; x3; x4]
+
+inline_for_extraction noextract
+let felem_list = x:list uint64{FL.length x == 5}
+inline_for_extraction noextract
+let point_list = x:list uint64{FL.length x == 20}
+
+inline_for_extraction noextract
+let pow51 = SF51.pow51
+
+[@"opaque_to_smt"]
+let pow102: (pow102:pos{pow2 102 == pow102 /\ pow102 = pow51 * pow51}) =
+  let pow102:pos = normalize_term (pow2 102) in
+  normalize_term_spec (pow2 102);
+  Math.Lemmas.pow2_plus 51 51;
+  pow102
+
+[@"opaque_to_smt"]
+let pow153: (pow153:pos{pow2 153 == pow153 /\ pow153 = pow51 * pow51 * pow51}) =
+  let pow153:pos = normalize_term (pow2 153) in
+  normalize_term_spec (pow2 153);
+  Math.Lemmas.pow2_plus 51 51;
+  Math.Lemmas.pow2_plus 102 51;
+  pow153
+
+[@"opaque_to_smt"]
+let pow204: (pow204:pos{pow2 204 == pow204 /\ pow204 = pow51 * pow51 * pow51 * pow51}) =
+  let pow204:pos = normalize_term (pow2 204) in
+  normalize_term_spec (pow2 204);
+  Math.Lemmas.pow2_plus 51 51;
+  Math.Lemmas.pow2_plus 102 51;
+  Math.Lemmas.pow2_plus 153 51;
+  pow204
+
+
+inline_for_extraction noextract
+let felem_to_list (x:SC.elem) : felem_list =
+  [@inline_let] let x0 = x % pow51 in
+  [@inline_let] let x1 = x / pow51 % pow51 in
+  [@inline_let] let x2 = x / pow102 % pow51 in
+  [@inline_let] let x3 = x / pow153 % pow51 in
+  [@inline_let] let x4 = x / pow204 in
+  Math.Lemmas.lemma_div_lt_nat x 255 204;
+  [@inline_let] let r = create5 (u64 x0) (u64 x1) (u64 x2) (u64 x3) (u64 x4) in
+  assert_norm (FL.length r = 5);
+  r
+
+
+inline_for_extraction noextract
+let ext_point_to_list (p:S.ext_point) : point_list =
+  [@inline_let] let (px, py, pz, pt) = p in
+  FL.(felem_to_list px @ felem_to_list py @ felem_to_list pz @ felem_to_list pt)
+
+//----------------------------------------------
+
+let create5_lseq (x0 x1 x2 x3 x4:uint64) : lseq uint64 5 =
+  let l = [x0; x1; x2; x3; x4] in
+  assert_norm (FL.length l = 5);
+  Seq.seq_of_list l
+
+
+val create5_lemma (x0 x1 x2 x3 x4:uint64) :
+  Lemma (let s = create5_lseq x0 x1 x2 x3 x4 in
+    s.[0] == x0 /\ s.[1] == x1 /\ s.[2] == x2 /\ s.[3] == x3 /\ s.[4] == x4)
+let create5_lemma x0 x1 x2 x3 x4 =
+  Seq.elim_of_list [x0; x1; x2; x3; x4]
+
+//-----------------------------------
+
+noextract
+let list_as_felem5 (f:felem_list) : SF51.felem5 =
+  let x = Seq.seq_of_list f <: lseq uint64 5 in
+  F51.lseq_as_felem x
+
+
+val felem_to_list_index_lemma: x:SC.elem ->
+  Lemma (let (f0, f1, f2, f3, f4) = list_as_felem5 (felem_to_list x) in
+    let x0 = x % pow51 in
+    let x1 = x / pow51 % pow51 in
+    let x2 = x / pow102 % pow51 in
+    let x3 = x / pow153 % pow51 in
+    let x4 = x / pow204 in
+    v f0 == x0 /\ v f1 == x1 /\ v f2 == x2 /\ v f3 == x3 /\ v f4 == x4)
+
+let felem_to_list_index_lemma x =
+  let x0 = x % pow51 in
+  let x1 = x / pow51 % pow51 in
+  let x2 = x / pow102 % pow51 in
+  let x3 = x / pow153 % pow51 in
+  let x4 = x / pow204 in
+  let f = felem_to_list x in
+
+  let (f0, f1, f2, f3, f4) = list_as_felem5 f in
+  Math.Lemmas.lemma_div_lt_nat x 255 204;
+  create5_lemma (u64 x0) (u64 x1) (u64 x2) (u64 x3) (u64 x4);
+  assert (v f0 == x0 /\ v f1 == x1 /\ v f2 == x2 /\ v f3 == x3 /\ v f4 == x4)
+
+
+val felem_to_list_lemma_fits: x:SC.elem ->
+  Lemma (SF51.felem_fits5 (list_as_felem5 (felem_to_list x)) (1, 1, 1, 1, 1))
+
+let felem_to_list_lemma_fits x =
+  felem_to_list_index_lemma x;
+  let x0 = x % pow51 in
+  let x1 = x / pow51 % pow51 in
+  let x2 = x / pow102 % pow51 in
+  let x3 = x / pow153 % pow51 in
+  let x4 = x / pow204 in
+  assert (SF51.felem_fits1 (u64 x0) 1);
+  assert (SF51.felem_fits1 (u64 x1) 1);
+  assert (SF51.felem_fits1 (u64 x2) 1);
+  assert (SF51.felem_fits1 (u64 x3) 1);
+  Math.Lemmas.lemma_div_lt_nat x 255 204;
+  assert (SF51.felem_fits1 (u64 x4) 1)
+
+
+val lemma_mod_pow2_sub: x:nat -> a:nat -> b:nat ->
+  Lemma (x / pow2 a % pow2 b * pow2 a == x % pow2 (a + b) - x % pow2 a)
+
+let lemma_mod_pow2_sub x a b =
+  calc (==) {
+    x / pow2 a % pow2 b * pow2 a;
+    (==) { Math.Lemmas.pow2_modulo_division_lemma_1 x a (a + b) }
+    x % pow2 (a + b) / pow2 a * pow2 a;
+    (==) { Math.Lemmas.euclidean_division_definition (x % pow2 (a + b)) (pow2 a) }
+    x % pow2 (a + b) - x % pow2 (a + b) % pow2 a;
+    (==) { Math.Lemmas.pow2_modulo_modulo_lemma_1 x a (a + b) }
+    x % pow2 (a + b) - x % pow2 a;
+  }
+
+
+val felem_to_list_lemma_eval: x:SC.elem ->
+  Lemma (SF51.as_nat5 (list_as_felem5 (felem_to_list x)) == x)
+
+let felem_to_list_lemma_eval x =
+  felem_to_list_index_lemma x;
+  let x0 = x % pow51 in
+  let x1 = x / pow51 % pow51 in
+  let x2 = x / pow102 % pow51 in
+  let x3 = x / pow153 % pow51 in
+  let x4 = x / pow204 in
+  let (f0, f1, f2, f3, f4) = list_as_felem5 (felem_to_list x) in
+  Math.Lemmas.lemma_div_lt_nat x 255 204;
+  let nat_x = SF51.as_nat5 (f0, f1, f2, f3, f4) in
+  assert (nat_x == x0 + x1 * pow51 + x2 * pow102 + x3 * pow153 + x4 * pow204);
+  calc (==) {
+    x0 + x1 * pow51 + x2 * pow102 + x3 * pow153 + x4 * pow204;
+    (==) { }
+    x0 + x1 * pow51 + x2 * pow102 + (x / pow153 % pow51) * pow153 + x / pow204 * pow204;
+    (==) { lemma_mod_pow2_sub x 153 51 }
+    x0 + x1 * pow51 + x2 * pow102 + x % pow204 - x % pow153 + x / pow204 * pow204;
+    (==) { Math.Lemmas.euclidean_division_definition x pow204 }
+    x0 + x1 * pow51 + (x / pow102 % pow51) * pow102 - x % pow153 + x;
+    (==) { lemma_mod_pow2_sub x 102 51 }
+    x0 + (x / pow51 % pow51) * pow51 - x % pow102 + x;
+    (==) { lemma_mod_pow2_sub x 51 51 }
+    x;
+  }
+
+//--------------------------------------------
+
+inline_for_extraction noextract
+let point_inv_list (p:point_list) =
+  let x = Seq.seq_of_list p <: lseq uint64 20 in
+  //F51.inv_ext_point x
+  F51.linv x
+
+noextract
+let point_eval_list (p:point_list) : GTot S.ext_point =
+  let x = Seq.seq_of_list p <: lseq uint64 20 in
+  F51.refl_ext_point x
+
+
+val ext_point_to_list_sub: p:S.ext_point -> Lemma
+ (let (px, py, pz, pt) = p in
+  let px_list = felem_to_list px in
+  let py_list = felem_to_list py in
+  let pz_list = felem_to_list pz in
+  let pt_list = felem_to_list pt in
+  let p_list = FL.(px_list @ py_list @ pz_list @ pt_list) in
+
+  let p_lseq = Seq.seq_of_list p_list <: lseq uint64 20 in
+  let px_lseq = Seq.seq_of_list px_list <: lseq uint64 5 in
+  let py_lseq = Seq.seq_of_list py_list <: lseq uint64 5 in
+  let pz_lseq = Seq.seq_of_list pz_list <: lseq uint64 5 in
+  let pt_lseq = Seq.seq_of_list pt_list <: lseq uint64 5 in
+  sub p_lseq 0 5 == px_lseq /\
+  sub p_lseq 5 5 == py_lseq /\
+  sub p_lseq 10 5 == pz_lseq /\
+  sub p_lseq 15 5 == pt_lseq)
+
+let ext_point_to_list_sub p =
+  let (px, py, pz, pt) = p in
+  let px_list = felem_to_list px in
+  let py_list = felem_to_list py in
+  let pz_list = felem_to_list pz in
+  let pt_list = felem_to_list pt in
+
+  FL.append_assoc px_list py_list pz_list;
+  assert (FL.(px_list @ py_list @ pz_list) ==
+    FL.append (FL.append px_list py_list) pz_list);
+
+  calc (==) { // ((a * b) * c) * d == a * (b * (c * d))
+    FL.append (FL.append (FL.append px_list py_list) pz_list) pt_list;
+    (==) { FL.append_assoc FL.(px_list @ py_list) pz_list pt_list }
+    FL.append (FL.append px_list py_list) (FL.append pz_list pt_list);
+    (==) { FL.append_assoc px_list py_list (FL.append pz_list pt_list) }
+    FL.(px_list @ py_list @ pz_list @ pt_list);
+  };
+
+  SPT.seq_of_list_append_lemma px_list py_list;
+  SPT.seq_of_list_append_lemma FL.(px_list @ py_list) pz_list;
+  SPT.seq_of_list_append_lemma FL.(px_list @ py_list @ pz_list) pt_list
+
+
+val ext_point_to_list_eval: p:S.ext_point ->
+  Lemma (point_eval_list (ext_point_to_list p) == p)
+
+let ext_point_to_list_eval p =
+  let (px, py, pz, pt) = p in
+  ext_point_to_list_sub p;
+  felem_to_list_lemma_eval px;
+  felem_to_list_lemma_eval py;
+  felem_to_list_lemma_eval pz;
+  felem_to_list_lemma_eval pt;
+  Math.Lemmas.small_mod px SC.prime;
+  Math.Lemmas.small_mod py SC.prime;
+  Math.Lemmas.small_mod pz SC.prime;
+  Math.Lemmas.small_mod pt SC.prime
+
+
+val ext_point_to_list_lemma: p:S.ext_point{Spec.Ed25519.point_inv p} ->
+  Lemma (point_inv_list (ext_point_to_list p) /\ point_eval_list (ext_point_to_list p) == p)
+
+let ext_point_to_list_lemma p =
+  ext_point_to_list_eval p;
+  let (px, py, pz, pt) = p in
+  ext_point_to_list_sub p;
+  felem_to_list_lemma_fits px;
+  felem_to_list_lemma_fits py;
+  felem_to_list_lemma_fits pz;
+  felem_to_list_lemma_fits pt
